\paragraph{And} \mbox{} \\
\AxiomC{$\Phi~prop~[\Gamma]$}
\AxiomC{$\Psi~prop~[\Gamma]$}
\RightLabel{$F-\wedge$}
\BinaryInfC{$\Phi~\wedge~\Psi~prop~[\Gamma]$}
\DisplayProof\qquad
\AxiomC{$a~\in~\Phi$}
\AxiomC{$b~\in~\Psi$}
\RightLabel{$I-\wedge$}
\BinaryInfC{$<a, b>~\in~\Phi~\wedge~\Psi~[\Gamma]$}
\DisplayProof

\vspace{0.2in}
\AxiomC{$p~\in~\Phi~\wedge~\Psi~[\Gamma]$}
\RightLabel{$E_1-\wedge$}
\UnaryInfC{$fst(p)~\in~B~[\Gamma]$}
\DisplayProof\qquad
\AxiomC{$p~\in~\Phi~\wedge~\Psi~[\Gamma]$}
\RightLabel{$E_2-\wedge$}
\UnaryInfC{$snd(p)~\in~C~[\Gamma]$}
\DisplayProof

\vspace{0.2in}
\AxiomC{$a~=~a'~\in~\Phi~[\Gamma]$}
\AxiomC{$b~=~b'~\in~\Psi~[\Gamma]$}
\RightLabel{$U_1-\wedge$}
\BinaryInfC{$<a,b>~=~<a',b'>~\in~\Phi~\wedge~\Psi~[\Gamma]$}
\DisplayProof

\vspace{0.2in}
\AxiomC{$p~=~q~\in~\Phi~\wedge~\Psi~[\Gamma]$}
\RightLabel{$U_2-\wedge$}
\UnaryInfC{$fst(p)~=~fst(q)~\in~\Phi~\wedge~\Psi~[\Gamma]$}
\DisplayProof\qquad
\AxiomC{$p~=~q~\in~\Phi~\wedge~\Psi~[\Gamma]$}
\RightLabel{$U_3-\wedge$}
\UnaryInfC{$snd(p)~=~snd(q)~\in~\Phi~\wedge~\Psi~[\Gamma]$}
\DisplayProof

\vspace{0.2in}
\AxiomC{$a~\in~\Phi~[\Gamma]$}
\AxiomC{$b~\in~\Psi~[\Gamma]$}
\RightLabel{$C_1-\wedge$}
\BinaryInfC{$fst(<a,b>)~=~a~\in~\Phi~[\Gamma]$}
\DisplayProof\qquad
\AxiomC{$a~\in~\Phi~[\Gamma]$}
\AxiomC{$b~\in~\Psi~[\Gamma]$}
\RightLabel{$C_2-\wedge$}
\BinaryInfC{$snd(<a,b>)~=~b~\in~\Psi~[\Gamma]$}
\DisplayProof

\paragraph{Or} \mbox{} \\
\AxiomC{$\Phi~prop~[\Gamma]$}
\AxiomC{$\Psi~prop~[\Gamma]$}
\RightLabel{$F-\vee$}
\BinaryInfC{$\Phi~\vee~\Psi~prop~[\Gamma]$}
\DisplayProof\qquad
\AxiomC{$a~\in~\Phi~[\Gamma]$}
\RightLabel{$I_1-\vee$}
\UnaryInfC{$inl(a)~\in~\Phi~\vee~\Psi~[\Gamma]$}
\DisplayProof\qquad
\AxiomC{$a~\in~\Psi~[\Gamma]$}
\RightLabel{$I_2-\vee$}
\UnaryInfC{$inr(a)~\in~\Phi~\vee~\Psi~[\Gamma]$}
\DisplayProof

\vspace{0.2in}
\AxiomC{$p~\in~\Phi~\vee~\Psi~[\Gamma]$}
\AxiomC{$X~prop~[\Gamma]$}
\AxiomC{$d(u)~\in~X~[\Gamma,~u~\in~\Phi]$}
\AxiomC{$c(w)~\in~X~[\Gamma,~w~\in~\Psi]$}
\RightLabel{$E-\vee$}
\QuaternaryInfC{$case(p,~(u).d,~(w).c)~\in~X~[\Gamma]$}
\DisplayProof

\vspace{0.2in}
\AxiomC{$a~=~a'~\in~\Phi~[\Gamma]$}
\RightLabel{$U_1-\vee$}
\UnaryInfC{$inl(a)~=~inl(a')~\in~\Phi~\vee~\Psi~[\Gamma]$}
\DisplayProof\qquad
\AxiomC{$b~=~b'~\in~\Psi~[\Gamma]$}
\RightLabel{$U_2-\vee$}
\UnaryInfC{$inr(b)~=~inr(b')~\in~\Phi~\vee~\Psi~[\Gamma]$}
\DisplayProof

\vspace{0.2in}
\AxiomC{$X~prop~[\Gamma]$}
\AxiomC{$p~=~q~\in~\Phi~\vee~\Psi~[\Gamma]$}
\AxiomC{$c(w)~=~d(u)~\in~X~[\Gamma,~w~\in~\Psi,~u~\in~\Phi]$}
\RightLabel{$U_3-\vee$}
\TrinaryInfC{$case(p,~(u).d,~(w).c)~=~case(q,~(u).d,~(w).c)~\in~\Phi~\vee~\Psi~[\Gamma]$}
\DisplayProof

\vspace{0.2in}
\AxiomC{$a~\in~\Phi~[\Gamma]$}
\AxiomC{$X~prop~[\Gamma]$}
\AxiomC{$d(u)~\in~X~[\Gamma,~u~\in~\Phi]$}
\AxiomC{$c(w)~\in~X~[\Gamma,~w~\in~\Psi]$}
\RightLabel{$C_1-\vee$}
\QuaternaryInfC{$case(inl(a),~(u).d,~(w).c)~=~d(u)~\in~\Phi~[\Gamma]$}
\DisplayProof

\vspace{0.2in}
\AxiomC{$b~\in~\Psi~[\Gamma]$}
\AxiomC{$X~prop~[\Gamma]$}
\AxiomC{$d(u)~\in~X~[\Gamma,~u~\in~\Phi]$}
\AxiomC{$c(w)~\in~X~[\Gamma,~w~\in~\Psi]$}
\RightLabel{$C_2-\vee$}
\QuaternaryInfC{$case(inr(b),~(u).d,~(w).c)~=~c(w)~\in~\Psi~[\Gamma]$}
\DisplayProof

\paragraph{Implicazione} \mbox{} \\
\AxiomC{$\Phi~prop~[\Gamma]$}
\AxiomC{$\Psi~prop~[\Gamma]$}
\RightLabel{$F-\to$}
\BinaryInfC{$\Phi~\to~\Psi~prop~[\Gamma]$}
\DisplayProof\qquad
\AxiomC{$b(u)~\in~\Psi~[\Gamma,~u~\in~\Phi]$}
\RightLabel{$I-\to$}
\UnaryInfC{$\lambda u.b(u)~\in~\Phi~\to~\Psi~[\Gamma]$}
\DisplayProof

\vspace{0.2in}
\AxiomC{$f~\in~\Phi~\to~\Psi~[\Gamma]$}
\AxiomC{$p~\in~\Phi~[\Gamma]$}
\RightLabel{$E-\to$}
\BinaryInfC{$Ap(f, p)~\in~\Psi~[\Gamma]$}
\DisplayProof\qquad
\AxiomC{$b(u)~=~b'(u)~\in~\Psi~[\Gamma,~u~\in~\Phi]$}
\RightLabel{$U_1-\to$}
\UnaryInfC{$\lambda u.b(u)~=~\lambda u.b'(u)~\in~\Phi~\to~\Psi~[\Gamma]$}
\DisplayProof

\vspace{0.2in}
\AxiomC{$f~=~f'~\in~\Phi~\to~\Psi~[\Gamma]$}
\AxiomC{$p~=~p'~\in~\Phi~[\Gamma]$}
\RightLabel{$U_2-\to$}
\BinaryInfC{$Ap(f, p)~=~Ap(f',p')~\in~\Psi~[\Gamma]$}
\DisplayProof

\vspace{0.2in}
\AxiomC{$a~\in~\Phi~[\Gamma]$}
\AxiomC{$b(u)~\in~\Psi~[\Gamma,~u~\in~\Phi]$}
\RightLabel{$C-\to$}
\BinaryInfC{$Ap(\lambda u.b(u),~a)~=~b(a)~\in~\Psi~[\Gamma]$}
\DisplayProof

\paragraph{Per ogni} \mbox{} \\
\AxiomC{$\Phi(x)~prop~[\Gamma,~x~\in~A]$}
\RightLabel{$F-\forall$}
\UnaryInfC{$(\forall x~\in~A)\Phi(x)~prop~[\Gamma]$}
\DisplayProof\qquad
\AxiomC{$A~type~[\Gamma]$}
\AxiomC{$b(w)~\in~\Phi(w)~[\Gamma,~w~\in~A]$}
\RightLabel{$I-\forall$}
\BinaryInfC{$\lambda w.b(w)~\in~(\forall x~\in~A)\Phi(x)~[\Gamma]$}
\DisplayProof

\vspace{0.2in}
\AxiomC{$A~type~[\Gamma]$}
\AxiomC{$f~\in~(\forall x~\in~A)\Phi(x)~[\Gamma]$}
\AxiomC{$t~\in~A~[\Gamma]$}
\RightLabel{$E-\forall$}
\TrinaryInfC{$Ap(f, t)~\in~\Phi(t)~[\Gamma]$}
\DisplayProof

\vspace{0.2in}
\AxiomC{$A~type~[\Gamma]$}
\AxiomC{$b(w)~=b'(w)~\in~\Phi(w)~[\Gamma,~w~\in~A]$}
\RightLabel{$U_1-\forall$}
\BinaryInfC{$\lambda w.b(w)~=~\lambda w.b'(w)~\in~(\forall x~\in~A)\Phi(x)~[\Gamma]$}
\DisplayProof

\vspace{0.2in}
\AxiomC{$A~type~[\Gamma]$}
\AxiomC{$f~=~f'~\in~(\forall x~\in~A)\Phi(x)~[\Gamma]$}
\AxiomC{$t~=~t'~\in~A~[\Gamma]$}
\RightLabel{$U_2-\forall$}
\TrinaryInfC{$Ap(f, t)~=~Ap(f',t')~\in~\Phi(t)~[\Gamma]$}
\DisplayProof

\vspace{0.2in}
\AxiomC{$A~type~[\Gamma]$}
\AxiomC{$t~\in~A~[\Gamma]$}
\AxiomC{$b(w)~\in~\Phi(w)~[\Gamma,~w~\in~A]$}
\RightLabel{$C-\forall$}
\TrinaryInfC{$Ap(\lambda w.b(w),~a)~=~b(a)~\in~\Phi(a)~[\Gamma]$}
\DisplayProof

\paragraph{Esiste} \mbox{} \\
\AxiomC{$\Phi(x)~prop~[\Gamma,~x~\in~A]$}
\RightLabel{$F-\exists$}
\UnaryInfC{$(\exists x~\in~A)\Phi(x)~prop~[\Gamma]$}
\DisplayProof\qquad
\AxiomC{$A~type~[\Gamma]$}
\AxiomC{$t~\in~A~[\Gamma]$}
\AxiomC{$p~\in~\Phi(t)~[\Gamma]$}
\RightLabel{$I-\exists$}
\TrinaryInfC{$<t, p>~\in~(\exists x~\in~A)\Phi(x)~[\Gamma]$}
\DisplayProof

\vspace{0.2in}
\AxiomC{$A~type~[\Gamma]$}
\AxiomC{$\Psi~prop~[\Gamma]$}
\AxiomC{$p~\in~(\exists x~\in~A)\Phi(x)~[\Gamma]$}
\AxiomC{$q(w,~y)~\in~\Psi~[\Gamma,~w~\in~A,~y~\in~\Phi(x)]$}
\RightLabel{$E-\exists$}
\QuaternaryInfC{$unpack(p, (w,~y)q)~\in~\Psi~[\Gamma]$}
\DisplayProof

\vspace{0.2in}
\AxiomC{$A~type~[\Gamma]$}
\AxiomC{$t~=~t'~\in~A~[\Gamma]$}
\AxiomC{$p~=~p'~\in~\Phi(t)~[\Gamma]$}
\RightLabel{$U_1-\exists$}
\TrinaryInfC{$unpack(<t, p>, )~=~<t',p'>~\in~(\exists x~\in~A)\Phi(x)~[\Gamma]$}
\DisplayProof

\begin{scriptsize}
	\vspace{0.2in}
	\AxiomC{$A~type~[\Gamma]$}
	\AxiomC{$\Psi~prop~[\Gamma]$}
	\AxiomC{$p~=~p'~\in~(\exists x~\in~A)\Phi(x)~[\Gamma]$}
	\AxiomC{$q(w,~y)~=~q'(w,~y)~\in~\Psi~[\Gamma,~w~\in~A,~y~\in~\Phi(x)]$}
	\RightLabel{$U_2-\exists$}
	\QuaternaryInfC{$unpack(p, (w,~y)q)~=~unpack(p', (w,~y)q')~\in~\Psi~[\Gamma]$}
	\DisplayProof
	
	\vspace{0.2in}
	\AxiomC{$A~type~[\Gamma]$}
	\AxiomC{$t~\in~A~[\Gamma]$}
	\AxiomC{$p~\in~\Phi(t)~[\Gamma]$}
	\AxiomC{$q(w,~y)~\in~\Psi~[\Gamma,~w~\in~A,~y~\in~\Phi(x)]$}
	\RightLabel{$C-\exists$}
	\QuaternaryInfC{$unpack(<t, p>, q)~=~q(t,p)~\in~\Psi~[\Gamma]$}
	\DisplayProof
\end{scriptsize}

\paragraph{Uguaglianza} \mbox{} \\
\AxiomC{$\Phi~prop~[\Gamma]$}
\AxiomC{$a~\in~\Psi~[\Gamma]$}
\AxiomC{$b~\in~\Psi~[\Gamma]$}
\RightLabel{$F-Id$}
\TrinaryInfC{$\Id(\Phi, a, b)~prop~[\Gamma]$}
\DisplayProof\qquad
\AxiomC{$a~\in~Phi$}
\RightLabel{$I-Id$}
\UnaryInfC{$id(a)~\in~Id(\Phi,a,a)~[\Gamma]$}
\DisplayProof
	
\begin{scriptsize}
	\vspace{0.2in}
	\AxiomC{$C(x,~y)~type~[\Gamma,~x~\in~\Phi,~y~\in~\Phi]$}
	\AxiomC{$a~\in~\Phi~[\Gamma]$}
	\AxiomC{$b~\in~\Phi~[\Gamma]$}
	\AxiomC{$p~\in~Id(\Phi,a,b)~[\Gamma]$}
	\AxiomC{$c(x)~\in~C(x,x)~[\Gamma,~x\in~\Phi]$}
	\RightLabel{$E-Id$}
	\QuinaryInfC{$El(p,~(x).c)~\in~C(a,b)~[\Gamma]$}
	\DisplayProof
\end{scriptsize}

\vspace{0.2in}
\AxiomC{$a~=~b~\in~\Phi~[\Gamma,~a\in~\Phi,~b\in~\Phi]$}
\RightLabel{$U_1-Id$}
\UnaryInfC{$id(a)~=~id(b)~\in~Id(\Phi,a,b)~[\Gamma,~a\in~\Phi,~b\in~\Phi]$}
\DisplayProof

\begin{scriptsize}
	\vspace{0.2in}
	\AxiomC{$C(x,~y)~type~[\Gamma,~x~\in~\Phi,~y~\in~\Phi]$}
	\AxiomC{$a~=~b~\in~\Phi~[\Gamma]$}
	\AxiomC{$p~=~q~\in~\Phi~=~\Phi~[\Gamma]$}
	\AxiomC{$c(x)~=~d(x)~\in~C(x,x)~[\Gamma,~x\in~\Phi,~c~\in~C(x,x),~d~\in~C(x,x)]$}
	\RightLabel{$U_2-Id$}
	\QuaternaryInfC{$El(p,~(a).c)=~sse(q,~(b).d)~\in~C(a,~p)~[\Gamma]$}
	\DisplayProof
	
	\vspace{0.2in}
	\AxiomC{$C(x,~y)~type~[\Gamma,~x~\in~\Phi,~y~\in~\Phi]$}
	\AxiomC{$a~\in~\Phi~[\Gamma]$}
	\AxiomC{$c(x)~\in~C(x,x)~[\Gamma,~x\in~\Phi]$}
	\RightLabel{$C-Id$}
	\TrinaryInfC{$El(id(a),~(x).c)~=c(a)~\in~C(a,a)~[\Gamma]$}
	\DisplayProof
\end{scriptsize}